more thoughts

theories/module.v
@@ -1,18 +1,19 @@
 Require Import refframe.base.
 
-Inductive steps {A B} (R : A → list B → A → Prop) : A → list (list B) → A → Prop :=
+Inductive steps {A B C} (R : A → option C → option B → A → Prop) : A → list (option C * option B) → A → Prop :=
 | steps_refl ρ :
     steps R ρ [] ρ
-| steps_l ρ1 ρ2 ρ3 κ κs :
-    R ρ1 κ ρ2 →
+| steps_l ρ1 ρ2 ρ3 ι κ κs :
+    R ρ1 ι κ ρ2 →
     steps R ρ2 κs ρ3 →
-    steps R ρ1 (κ :: κs) ρ3.
+    steps R ρ1 ((ι, κ) :: κs) ρ3.
 
 Record module := {
   m_state : Type;
-  m_event : Type;
+  m_in_event : Type;
+  m_out_event : Type;
   m_initial : m_state → Prop;
-  m_step : m_state → list m_event → m_state → Prop;
+  m_step : m_state → option m_in_event → option m_out_event → m_state → Prop;
   (* This cannot be defined based on m_step since m_state might e.g. contain a threadpool
      and a state should be bad if any thread is stuck. *)
   m_good : m_state → Prop;
@@ -21,71 +22,92 @@ Record module := {
 Definition safe (m : module) : Prop :=
   ∀ σ κ σ', m.(m_initial) σ → steps m.(m_step) σ κ σ' → m.(m_good) σ'.
 
-Record refines (mimpl mspec : module) (trans_initial : mimpl.(m_state) → mspec.(m_state)) (trans_event : list mimpl.(m_event) → list mspec.(m_event)) := {
-  ref_initial σ : mimpl.(m_initial) σ → mspec.(m_initial) (trans_initial σ);
+Record refines (mimpl mspec : module) (ti : mimpl.(m_state) → mspec.(m_state)) (tin : mimpl.(m_in_event) → mspec.(m_in_event)) (tout : mimpl.(m_out_event) → mspec.(m_out_event)) := {
+  ref_initial σ : mimpl.(m_initial) σ → mspec.(m_initial) (ti σ);
   ref_step σ κ σi:
     mimpl.(m_initial) σ →
     steps mimpl.(m_step) σ κ σi →
-    (∀ σs, steps mspec.(m_step) (trans_initial σ) (trans_event <$> κ) σs → mspec.(m_good) σs) →
-    mimpl.(m_good) σi ∧ ∃ σs, steps mspec.(m_step) (trans_initial σ) (trans_event <$> κ) σs;
+    (∀ σs, steps mspec.(m_step) (ti σ) (prod_map (fmap tin) (fmap tout) <$> κ) σs → mspec.(m_good) σs) →
+    mimpl.(m_good) σi ∧ ∃ σs, steps mspec.(m_step) (ti σ) (prod_map (fmap tin) (fmap tout) <$> κ) σs;
 }.
 
-Lemma refines_preserves_safe mspec mimpl ti te:
+Lemma refines_preserves_safe mspec mimpl ti tin tout:
   safe mspec →
-  refines mimpl mspec ti te →
+  refines mimpl mspec ti tin tout →
   safe mimpl.
 Proof.
   move => Hs Hr σ κ σ' Hinit Hstep.
-  have [|]:= (ref_step _ _ _ _ Hr _ _ _ Hinit Hstep) => //.
+  have [|]:= (ref_step _ _ _ _ _ Hr _ _ _ Hinit Hstep) => //.
   move => σs Hsteps. apply: Hs => //.
   by apply: ref_initial.
 Qed.
 
-Lemma refines_reflexive m:
-  refines m m id id.
-Proof. constructor => // σ κ σi Hi Hs. rewrite list_fmap_id. naive_solver. Qed.
+Lemma prod_map_fmap_id {A B} (l : list (option A * option B)):
+  (prod_map (fmap id) (fmap id) <$> l) = l.
+Proof. rewrite -{2}(list_fmap_id l). apply list_fmap_ext => // -[[?|] [?|]] //. Qed.
 
-Lemma refines_vertical m1 m2 m3 ti1 te1 ti2 te2:
-  refines m1 m2 ti1 te1 →
-  refines m2 m3 ti2 te2 →
-  refines m1 m3 (ti2 ∘ ti1) (te2 ∘ te1).
+Lemma refines_reflexive m:
+  refines m m id id id.
+Proof. constructor => // σ κ σi Hi Hs. rewrite prod_map_fmap_id. naive_solver. Qed.
+
+Lemma prod_map_fmap_compose {A B C D E F} (f1 : A → B) (f2 : B → C) (g1 : D → E) (g2 : E → F) (l : list (option _ * option _)):
+  (prod_map (fmap (f2 ∘ f1)) (fmap (g2 ∘ g1)) <$> l) =
+  (prod_map (fmap f2) (fmap g2) <$> (prod_map (fmap f1) (fmap g1) <$> l)).
+Proof. rewrite -list_fmap_compose. apply list_fmap_ext => // -[[?|] [?|]] //. Qed.
+
+Lemma refines_vertical m1 m2 m3 ti1 tin1 tout1 ti2 tin2 tout2:
+  refines m1 m2 ti1 tin1 tout1 →
+  refines m2 m3 ti2 tin2 tout2 →
+  refines m1 m3 (ti2 ∘ ti1) (tin2 ∘ tin1) (tout2 ∘ tout1).
 Proof.
   move => Hr1 Hr2.
   constructor; first by destruct Hr1, Hr2; eauto.
-  move => σ κ σi Hinit1 Hstep1 /=. rewrite list_fmap_compose => Hsafe3.
-  have [|Hgood [σ2 Hstep2]] := (ref_step _ _ _ _ Hr1 _ _ _ Hinit1 Hstep1). {
+  move => σ κ σi Hinit1 Hstep1 /=. rewrite prod_map_fmap_compose => Hsafe3.
+  have [|Hgood [σ2 Hstep2]] := (ref_step _ _ _ _ _ Hr1 _ _ _ Hinit1 Hstep1). {
     move => σs2 Hstep2.
-    by have [||? _] := (ref_step _ _ _ _ Hr2 _ _ _ _ Hstep2); eauto using ref_initial.
+    by have [||? _] := (ref_step _ _ _ _ _ Hr2 _ _ _ _ Hstep2); eauto using ref_initial.
   }
   split => //.
-  have [||_ [σ3 Hstep3]] := (ref_step _ _ _ _ Hr2 _ _ _ _ Hstep2); eauto using ref_initial.
+  have [||_ [σ3 Hstep3]] := (ref_step _ _ _ _ _ Hr2 _ _ _ _ Hstep2); eauto using ref_initial.
 Qed.
 
-Inductive module_product_step (m1 m2 : module) : m1.(m_state) * m2.(m_state) → list (m1.(m_event) + m2.(m_event)) → m1.(m_state) * m2.(m_state) → Prop :=
-| ModuleStepBoth σ1 σ2 κs1 κs2 σ1' σ2' :
-    m1.(m_step) σ1 κs1 σ1' →
-    m2.(m_step) σ2 κs2 σ2' →
-    module_product_step m1 m2 (σ1, σ2) ((inl <$> κs1) ++ (inr <$> κs2)) (σ1', σ2)
-| ModuleStepLeft σ1 σ2 κs σ1' :
-    m1.(m_step) σ1 κs σ1' →
-    module_product_step m1 m2 (σ1, σ2) (inl <$> κs) (σ1', σ2)
-| ModuleStepRight σ1 σ2 κs σ2' :
-    m2.(m_step) σ2 κs σ2' →
-    module_product_step m1 m2 (σ1, σ2) (inr <$> κs) (σ1, σ2')
+Definition handles_call {A B} (in_event : option A) (out_event : option B) (r : A → B → Prop) : Prop :=
+  ∃ eo ei, in_event = Some ei ∧ out_event = Some eo ∧ r ei eo.
+
+Inductive module_product_step (m1 m2 : module) (r1 : m1.(m_in_event) → m2.(m_out_event) → Prop) (r2 : m2.(m_in_event) → m1.(m_out_event) → Prop) : m1.(m_state) * m2.(m_state) → option (m1.(m_in_event) + m2.(m_in_event)) → option (m1.(m_out_event) + m2.(m_out_event)) → m1.(m_state) * m2.(m_state) → Prop :=
+| ModuleStepBoth σ1 σ2 κs1 κs2 ι1 ι2 σ1' σ2' :
+    m1.(m_step) σ1 ι1 κs1 σ1' →
+    m2.(m_step) σ2 ι2 κs2 σ2' →
+    (* This means either m1 must be calling m2 or the other way around. *)
+       (ι2 = None ∧ handles_call ι1 κs2 r1)
+    ∨ (ι1 = None ∧ handles_call ι2 κs1 r2) →
+    module_product_step m1 m2 r1 r2 (σ1, σ2) None None (σ1', σ2)
+| ModuleStepLeft σ1 σ2 ι κs σ1' :
+    m1.(m_step) σ1 ι κs σ1' →
+    module_product_step m1 m2 r1 r2 (σ1, σ2) (inl <$> ι) (inl <$> κs) (σ1', σ2)
+| ModuleStepRight σ1 σ2 ι κs σ2' :
+    m2.(m_step) σ2 ι κs σ2' →
+    module_product_step m1 m2 r1 r2 (σ1, σ2) (inr <$> ι) (inr <$> κs) (σ1, σ2')
 .
 
-Definition module_product (m1 m2 : module) : module := {|
+Definition module_product (m1 m2 : module) (r1 : m1.(m_in_event) → m2.(m_out_event) → Prop) (r2 : m2.(m_in_event) → m1.(m_out_event) → Prop) : module := {|
   m_state := m1.(m_state) * m2.(m_state);
-  m_event := m1.(m_event) + m2.(m_event);
+  m_in_event := m1.(m_in_event) + m2.(m_in_event);
+  m_out_event := m1.(m_out_event) + m2.(m_out_event);
   m_initial σ := m1.(m_initial) σ.1 ∧ m2.(m_initial) σ.2;
-  m_step := module_product_step m1 m2;
+  m_step := module_product_step m1 m2 r1 r2;
   m_good σ := m1.(m_good) σ.1 ∧ m2.(m_good) σ.2;
 |}.
 
-
-
-
-
+Lemma refines_horizontal m1 m2 m1' m2' ti1 tin1 tout1 ti2 tin2 tout2 r1 r2 r1' r2':
+  refines m1 m1' ti1 tin1 tout1 →
+  refines m2 m2' ti2 tin2 tout2 →
+  refines (module_product m1 m2 r1 r2) (module_product m1' m2' r1' r2') (prod_map ti1 ti2) (sum_map tin1 tin2) (sum_map tout1 tout2).
+Proof.
+  move => Hr1 Hr2. constructor; first by move => [??]/= [??]; eauto using ref_initial.
+  move => /= [σ1 σ2] κ [σi1 σi2] /= [Hinit1 Hinit2].
+  have := (ref_step _ _ _ _ _ Hr1 _ _ _ Hinit1).
+Abort.
 
 (*
   Example:
@@ -109,40 +131,60 @@ Definition module_product (m1 m2 : module) : module := {|
                            Res 1
        Initial state  -------------->  Final State
 
+    out_event: Res Z
+
   Spec 1:                      Spec 2:
                                (no main)
    main: let x := Call A;       A: return 1
-         Emit (Res x)
+         Emit (Res x + 1)
+
+   out_event: Res Z | CallA    in_event: CallA
+     | RetA Z                  out_event: RetA Z
 
   Impl 1 High:                                    Memory High:
 
-   main: int* x = alloc_int;                      No offset operation on locations,
-         Call A x;                                Memory layout is hidden (i.e. integers are stored aso
-         Emit (Res *x)                            mathematical integers, constraint that all integers on the
-                                                  heap are 0 ≤ n < 2 ^ 32
+   main: int* x1 = alloc_int;                      No offset operation on locations,
+         int* x2 = alloc_int;                      Memory layout is hidden (i.e. integers are stored as
+         x2 := 1;                                  mathematical integers, constraint that all integers on the
+         Call A x1;                                heap are 0 ≤ n < 2 ^ 32
+         Emit (Res *x1 * *x2)
+
+   out_event: Res Z | CallA loc                   in_event: AllocInt loc | LoadInt loc Z | WriteInt loc Z
+     | RetA | AllocInt loc
+     | LoadInt loc Z
 
   Impl 1 Low:                  Impl 2 Low:        Memory Low:
 
-   main: int* x = alloc_int;   A p: *(p + 0) = 1; Flat memory model which stores bytes
-         Call A x;                  *(p + 1) = 0;
-         Emit (Res load_int(x))     *(p + 2) = 0;
-                                    *(p + 3) = 0;
+   main: int* x1 = alloc_int;   A p: (p + 0) := 1; Flat memory model which stores bytes
+         int* x2 = alloc_int;        (p + 1) := 0;
+         x2 := 1;                    (p + 2) := 0;
+         Call A x1;                  (p + 3) := 0;
+         Emit (Res *x1 + *x2)
+
+
+   out_event: Res Z | CallA loc in_event: CallA loc  in_event: AllocInt loc | WriteByte loc Z
+     | RetA | AllocInt loc      out_event: RetA         | LoadInt loc Z | WriteInt loc Z
+     | LoadInt loc Z              | WriteByte loc Z
+     | WriteInt loc Z
 
   Low level code (i.e. code with inline assembly)
-   main: int* x = alloc_int;     Flat memory model which stores bytes
-         *(x + 0) = 1;
-         *(x + 1) = 0;
-         *(x + 1) = 0;
-         *(x + 1) = 0;
-         Emit (Res load_int(x))
+   main: int* x1 = alloc_int;     Flat memory model which stores bytes
+         int* x2 = alloc_int;
+         x2 := 1;
+         (x1 + 0) := 1;
+         (x1 + 1) := 0;
+         (x1 + 1) := 0;
+         (x1 + 1) := 0;
+         Emit (Res *x1 + *x2)
 
+   out_event: Res Z
 
  Proofs:
 
   m1 < m2 : [refines m1 m2]
   m1 + m2 : [module_product m1 m2]
 
-  1: LLC < Impl 1 Low + Memory Low + Impl 2
+  1: LLC < Impl 1 Low + Memory Low + Impl 2 / {CallA, RetA, AllocInt, ...}
 
   2: Impl 1 Low | Memory Low < Impl 1 High | Memory High
 
